theories/Alpha/RenameApart_VarP.v
@@ -3,29 +3,19 @@ Require Import StableFresh.
 Require Import IL VarP RenameApart.
 
 
-Inductive FreshGenVarProp (P:var -> Prop) (FG:FreshGen) : Prop :=
-  {
-    fresh_var_inv : forall x, P (fst (fresh FG x));
-    fresh_var_list_inv : forall Z x, x ∈ of_list (fst (fresh_list FG Z)) -> P x;
-    fresh_inv : forall x, FreshGenVarProp P (snd (fresh FG x));
-    fresh_list_inv : forall Z, FreshGenVarProp P (snd (fresh_list FG Z));
-  }.
-
-Local Hint Resolve fresh_inv fresh_list_inv.
-
-Lemma renameApart_var_P (fresh:FreshGen) (P:var -> Prop) (ϱ:env var) s
-      (FGVP:FreshGenVarProp P fresh) (FGI:FreshGenVarProp P fresh)
+Lemma renameApart_var_P Fi (FG:FreshGen Fi) (FGS:FreshGenSpec FG) fi (P:var -> Prop) (ϱ:env var) s
+      (Pfresh:forall fi x, P (fst (fresh FG fi x)))
+      (Pfresh_list:forall fi Z, forall (x:var), x ∈ of_list (fst (fresh_list FG fi Z)) -> P x)
       (ren:forall x, x ∈ freeVars s -> P (ϱ x))
-  : var_P P (snd (renameApart' fresh ϱ s)).
+  : var_P P (snd (renameApart' FG fi ϱ s)).
 Proof.
-  revert ϱ ren fresh fresh FGVP FGI.
+  revert ϱ ren fi.
   induction s using stmt_ind'; intros; simpl;
     repeat let_pair_case_eq; repeat simpl_pair_eqs; subst; simpl in *.
   - econstructor; eauto.
     + eapply IHs; eauto.
-      * intros; lud; eauto using fresh_var_inv. eapply fresh_var_inv. eauto.
+      * intros; lud; eauto.
         eapply ren. cset_tac.
-    + eapply fresh_var_inv; eauto.
     + rewrite freeVars_renameExp. unfold lookup_set.
       hnf; intros. cset_tac.
   - econstructor; eauto.
@@ -33,7 +23,6 @@ Proof.
       hnf; intros. cset_tac.
     + eapply IHs1; eauto. cset_tac.
     + eapply IHs2; eauto. cset_tac.
-
   - econstructor.
     rewrite freeVars_rename_op_list. unfold lookup_set.
     hnf; intros. cset_tac.
@@ -44,13 +33,13 @@ Proof.
     + intros. inv_get.
       edestruct get_fst_renameApartF as [? [? ?]]; eauto; dcr; subst.
       destruct Zs as [Z s']; simpl in *; subst.
-      eapply IH; eauto.
+      eapply H; eauto.
       intros. decide (x ∈ of_list (fst x0)).
       * edestruct update_with_list_lookup_in_list; try eapply i; dcr.
         Focus 2.
-        rewrite H11.
-        exploit fresh_list_stable_get; try eapply H10; eauto; dcr.
-        subst. get_functional. eapply freshP; eauto.
+        rewrite H6.
+        eapply get_in_of_list in H5.
+        eapply Pfresh_list; eauto.
         eauto with len.
       * rewrite lookup_set_update_not_in_Z; eauto.
         eapply ren.
@@ -62,8 +51,7 @@ Proof.
       edestruct get_fst_renameApartF as [? [? ?]]; eauto; dcr; subst.
       destruct Zs as [Z s']; simpl in *; subst.
       hnf; intros.
-      eapply fresh_list_stable_In in H0; dcr; subst.
-      eapply freshP.
-    + eapply IH; eauto.
+      eapply Pfresh_list; eauto.
+    + eapply IHs; eauto.
       cset_tac.
 Qed.
